Simplify

Semantics/Imp/Aexp.lean
@@ -15,12 +15,12 @@ private inductive BigStep: Aexp × State -> Int -> Prop
 
 infix:10 " ==> " => BigStep
 
-private instance BigStep.equiv: Setoid Aexp where
+private instance equiv: Setoid Aexp where
   r a a' := ∀{s n}, ((a, s) ==> n) = ((a', s) ==> n)
   iseqv := {
     refl := fun _ => rfl
     symm := (Eq.symm .)
-    trans := (. ▸ .)
+    trans := (Eq.rec . .)
   }
 
 private example: ((var "x" + 5) + (9 - 7), s0) ==> 7 :=
@@ -38,14 +38,14 @@ def reduce (a: Aexp) (s: State): Int :=
   | sub a a' => reduce a s - reduce a' s
   | mul a a' => reduce a s * reduce a' s
 
-instance: CoeFun Aexp (fun _ => State -> Int) := CoeFun.mk reduce
+instance: CoeFun Aexp (fun _a => State -> Int) := ⟨reduce⟩
 
 instance reduce.equiv: Setoid Aexp where
   r a a' := ∀{s}, a s = a' s
   iseqv := {
     refl := fun _ => rfl
     symm := fun h => h.symm
-    trans := fun h1 h2 => h1 ▸ h2
+    trans := fun h1 h2 => h2.rec h1
   }
 
 #eval ((var "x" + 5) + (9 - 7)) s0 -- 7
@@ -56,43 +56,40 @@ section Equivalence
 private theorem reduce.from_natural
   (hBigStep: conf ==> n): conf.1 conf.2 = n :=
   by induction hBigStep with
-  | add _ _ iha iha' => exact iha ▸ iha' ▸ rfl
-  | sub _ _ iha iha' => exact iha ▸ iha' ▸ rfl
-  | mul _ _ iha iha' => exact iha ▸ iha' ▸ rfl
+  | add _ _ iha iha' => exact iha.rec $ iha'.rec rfl
+  | sub _ _ iha iha' => exact iha.rec $ iha'.rec rfl
+  | mul _ _ iha iha' => exact iha.rec $ iha'.rec rfl
   | _ => rfl
 
 private theorem BigStep.from_reduce
   (hred: a s = n): (a, s) ==> n :=
   by induction a generalizing n with
-  | val a => exact hred ▸ BigStep.val
-  | var a => exact hred ▸ BigStep.var
+  | val a => exact hred.rec BigStep.val
+  | var a => exact hred.rec BigStep.var
   | add a a' iha iha' =>
-    exact hred ▸ BigStep.add (iha rfl) (iha' rfl)
+    exact hred.rec (iha rfl).add (iha' rfl)
   | sub a a' iha iha' =>
-    exact hred ▸ BigStep.sub (iha rfl) (iha' rfl)
+    exact hred.rec (iha rfl).sub (iha' rfl)
   | mul a a' iha iha' =>
-    exact hred ▸ BigStep.mul (iha rfl) (iha' rfl)
+    exact hred.rec (iha rfl).mul (iha' rfl)
 
 private theorem BigStep_eq_reduce:
   ((a, s) ==> n) = (a s = n) :=
-  propext (Iff.intro reduce.from_natural BigStep.from_reduce)
+  propext ⟨reduce.from_natural, BigStep.from_reduce⟩
 
 private theorem BigStep_eq_reduce':
   (a, s) ==> a s :=
   BigStep.from_reduce rfl
 
 private theorem BigStep_eq_eq_reduce_eq:
-  BigStep.BigStep.equiv.r a a' <-> reduce.equiv.r a a' := by
+  BigStep.equiv.r b b' <-> reduce.equiv.r b b' := by
   simp only [Setoid.r, eq_iff_iff]
   constructor
-  . intro h s
-    specialize @h s (a' s)
-    rw [BigStep_eq_reduce, BigStep_eq_reduce, eq_self, iff_true] at h
-    exact h
-  . intro h s _
-    rw [BigStep_eq_reduce, BigStep_eq_reduce]
-    specialize @h s
-    rw [h]
+  . exact fun h => Iff.mpr (BigStep_eq_reduce.rec h) (Eq.mpr BigStep_eq_reduce rfl)
+  . exact fun h => {
+      mp := fun h1 => (h ▸ (BigStep_eq_reduce ▸ h1)).rec BigStep_eq_reduce',
+      mpr := fun h1 => (h ▸ (BigStep_eq_reduce ▸ h1)).rec BigStep_eq_reduce'
+    }
 
 end Equivalence
 
