Semantics/Set.lean
@@ -8,7 +8,7 @@ namespace Set
 
 protected def Mem (s: Set α) (a: α): Prop := s a
 
-instance: Membership α (Set α) := Membership.mk Set.Mem
+instance: Membership α (Set α) := ⟨Set.Mem⟩
 
 theorem ext {a b: Set α} (h: ∀(x: α), x ∈ a <-> x ∈ b): a = b :=
   funext fun x => propext (h x)
@@ -16,11 +16,11 @@ theorem ext {a b: Set α} (h: ∀(x: α), x ∈ a <-> x ∈ b): a = b :=
 protected def Subset (a b: Set α) :=
   ∀{{x}}, x ∈ a -> x ∈ b
 
-instance: LE (Set α) := LE.mk Set.Subset
+instance: HasSubset (Set α) := ⟨Set.Subset⟩
 
-instance: HasSubset (Set α) := HasSubset.mk (. <= .)
+instance: LE (Set α) := ⟨(. ⊆ .)⟩
 
-instance: EmptyCollection (Set α) := EmptyCollection.mk fun _ => False
+instance: EmptyCollection (Set α) := ⟨fun _ => False⟩
 
 notation (priority := high) "{" x " | " p "}" => setOf fun x => p
 
@@ -28,25 +28,25 @@ def univ: Set α := {_ | True}
 
 protected def insert (a: α) (s: Set α): Set α := {x | x = a ∨ x ∈ s}
 
-instance: Insert α (Set α) := Insert.mk Set.insert
+instance: Insert α (Set α) := ⟨Set.insert⟩
 
 protected def singleton (a: α): Set α := {b | b = a}
 
-instance instSingletonSet: Singleton α (Set α) := Singleton.mk Set.singleton
+instance instSingletonSet: Singleton α (Set α) := ⟨Set.singleton⟩
 
 protected def union (a b: Set α): Set α := {x | x ∈ a ∨ x ∈ b}
 
-instance: Union (Set α) := Union.mk Set.union
+instance: Union (Set α) := ⟨Set.union⟩
 
 protected def inter (a b: Set α): Set α := {x | x ∈ a ∧ x ∈ b}
 
-instance: Inter (Set α) := Inter.mk Set.inter
+instance: Inter (Set α) := ⟨Set.inter⟩
 
 protected def compl (s: Set α): Set α := {a | a ∉ s}
 
 protected def diff (a b: Set α): Set α := {x | x ∈ a ∧ x ∉ b}
 
-instance: SDiff (Set α) := SDiff.mk Set.diff
+instance: SDiff (Set α) := ⟨Set.diff⟩
 
 end Set
 
@@ -70,7 +70,7 @@ theorem Subset.trans {a b c: Set α} (hab: a ⊆ b) (hbc: b ⊆ c): a ⊆ c :=
   fun _ h => hbc (hab h)
 
 theorem Subset.antisymm {a b: Set α} (hab: a ⊆ b) (hba: b ⊆ a): a = b :=
-  funext fun _ => propext (Iff.intro (fun mp => hab mp) (fun mp => hba mp))
+  funext fun _ => propext ⟨(hab .), (hba .)⟩
 
 theorem Subset.from_eq {a b: Set α} (heq: a = b): a ⊆ b :=
   fun _x hxa => heq ▸ hxa
@@ -82,10 +82,10 @@ theorem Subset.from_eq {a b: Set α} (heq: a = b): a ⊆ b :=
 def Set.ite (t a b: Set α): Set α := a ∩ t ∪ b \ t
 
 theorem Set.ite_mono (t: Set α) (hab: a ⊆ b) (hab': a' ⊆ b'):
-  ite t a a' ⊆ ite t b b' := fun _ h2 =>
-  match h2 with
-  | Or.inl (And.intro hl hr) => Or.inl (And.intro (hab hl) hr)
-  | Or.inr (And.intro hl hr) => Or.inr (And.intro (hab' hl) hr)
+  ite t a a' ⊆ ite t b b' := fun _ hite =>
+  match hite with
+  | Or.inl ⟨hl, hr⟩ => Or.inl ⟨hab hl, hr⟩
+  | Or.inr ⟨hl, hr⟩ => Or.inr ⟨hab' hl, hr⟩
 
 /-
   ## Set theoretic (partial) functions
@@ -103,7 +103,7 @@ theorem mem_id: (a, b) ∈ id <-> a = b :=
   Iff.rfl
 
 def comp (f g: α ->s α): α ->s α :=
-  {x | ∃z, (x.1, z) ∈ f ∧ (z, x.2) ∈ g}
+  {(x, y) | ∃z, (x, z) ∈ f ∧ (z, y) ∈ g}
 
 infixl:90 " ○ " => SFun.comp
 
@@ -111,24 +111,16 @@ theorem mem_comp: x ∈ f ○ g <-> ∃z, (x.1, z) ∈ f ∧ (z, x.2) ∈ g :=
   Iff.rfl
 
 theorem comp_mono (hfh: f ⊆ h) (hgk: g ⊆ k): f ○ g ⊆ h ○ k :=
-  fun _ (Exists.intro z (And.intro hl hr)) =>
-    Exists.intro z (And.intro (hfh hl) (hgk hr))
+  fun _ ⟨z, hl, hr⟩ => ⟨z, hfh hl, hgk hr⟩
 
-theorem comp_id: f ○ id = f := by
-  apply funext
-  intro (_x, y)
-  apply propext
-  constructor
-  . intro (Exists.intro z (And.intro hl hr))
-    apply mem_id.mp hr ▸ hl
-  . exact fun mp => (Exists.intro y (And.intro mp rfl))
+theorem comp_id: f ○ id = f := funext fun (_x, y) => propext {
+  mp := fun ⟨_z, hl, hr⟩ => mem_id.mp hr ▸ hl,
+  mpr := (⟨y, ., rfl⟩)
+}
 
-theorem id_comp: id ○ f = f := by
-  funext (x, _y)
-  apply propext
-  constructor
-  . intro (Exists.intro z (And.intro hl hr))
-    apply mem_id.mp hl ▸ hr
-  . exact fun mp => (Exists.intro x (And.intro rfl mp))
+theorem id_comp: id ○ f = f := funext fun (x, _y) => propext {
+  mp := fun ⟨_z, hl, hr⟩ => mem_id.mp hl ▸ hr,
+  mpr := (⟨x, rfl, .⟩)
+}
 
 end SFun
