Semantics/Imp/SmallStep.lean
@@ -31,17 +31,14 @@ private example:
 
 theorem cat_eq:
   ((c++c'', s) ~> conf)
-    = ((∃c' s', ((c, s) ~> (c', s')) ∧ conf = (c'++c'', s'))
-      ∨ (c = skip ∧ conf = (c'', s))) :=
-  propext {
+    <-> ((∃c' s', ((c, s) ~> (c', s')) ∧ conf = (c'++c'', s'))
+      ∨ (c = skip ∧ conf = (c'', s))) := {
     mp := fun hmp => match hmp with
-      | skipCat => Or.inr (And.intro rfl rfl)
-      | cat h =>
-        Or.inl (Exists.intro _ (Exists.intro _ (And.intro h rfl))),
+      | skipCat => Or.inr ⟨rfl, rfl⟩
+      | cat h => Or.inl ⟨_, _, h, rfl⟩,
     mpr := fun hmpr => match hmpr with
-      | Or.inl (Exists.intro _c' (Exists.intro _s' (And.intro hl hr))) =>
-        hr ▸ cat hl
-      | Or.inr (And.intro hl hr) => hl ▸ hr ▸ skipCat
+      | Or.inl ⟨_c', _s', hl, hr⟩ => hr ▸ cat hl
+      | Or.inr ⟨hl, hr⟩ => hl ▸ hr ▸ skipCat
   }
 
 theorem cond_eq:
@@ -49,13 +46,13 @@ theorem cond_eq:
     = (b s ∧ conf = (c, s) ∨ b s = false ∧ conf = (c', s)) :=
   propext {
     mp := fun hmp => match hb: b s with
-      | false => match hmp with | ifElse => Or.inr (And.intro rfl (hb ▸ rfl))
-      | true => match hmp with | ifElse => Or.inl (And.intro rfl (hb ▸ rfl)),
+      | false => match hmp with | ifElse => Or.inr ⟨rfl, hb ▸ rfl⟩
+      | true => match hmp with | ifElse => Or.inl ⟨rfl, hb ▸ rfl⟩,
     mpr := fun hmpr =>
       let hss: conf = (bif b s then c else c', s) :=
         match hb: b s with
-        | true => match hb ▸ hmpr with | Or.inl (And.intro _ hr) => hr
-        | false => match hb ▸ hmpr with | Or.inr (And.intro _ hr) => hr
+        | true => match hb ▸ hmpr with | Or.inl ⟨_, hr⟩ => hr
+        | false => match hb ▸ hmpr with | Or.inr ⟨_, hr⟩ => hr
       hss ▸ ifElse
   }
 
@@ -63,21 +60,34 @@ theorem cond_false (hb: b s = false):
   ((if b then c else c' end, s) ~> conf) = (conf = (c', s)) :=
   propext {
     mp := fun hmp => match hb ▸ cond_eq ▸ hmp with
-      | Or.inr (And.intro _ hr) => hr,
-    mpr := fun mp => cond_eq ▸ Or.inr (And.intro hb mp)
+      | Or.inr ⟨_, hr⟩ => hr,
+    mpr := fun mp => cond_eq ▸ Or.inr ⟨hb, mp⟩
   }
 
 infixl:10 " ~>* " => ReflTrans SmallStep
 
-theorem star.demo':
-  ([|x := 2; while 0 <= x loop x := x + 1 end|], s0) ~>*
-      ([|while 0 <= x loop x := x + 1 end|], s0["x" <- 2]) :=
-  ReflTrans.head (cat ass) (ReflTrans.head skipCat ReflTrans.refl)
+private example:
+  ([|x := 1; while x <= 1 loop x := x + 1 end|], s0) ~>*
+      (skip, s0["x" <- 1]["x" <- 2]) := by
+  apply ReflTrans.head (cat ass) (ReflTrans.head skipCat _)
+  apply ReflTrans.head whileLoop
+  have hs : s0["x" <- Aexp.reduce 1 s0] = s0["x" <- 1] := rfl
+  have hcond : (Bexp.le (Aexp.var "x") 1) (s0["x" <- 1]) = true := rfl
+  rw [hs, hcond]
+  simp
+  apply ReflTrans.head (cat ass)
+  apply ReflTrans.head skipCat
+  apply ReflTrans.head whileLoop
+  have hs : s0["x" <- 1]["x" <- (Aexp.var "x" + 1) (s0["x" <- 1])] = s0["x" <- 1]["x" <- 2] := rfl
+  have hcond : (Bexp.le (Aexp.var "x") 1) (s0["x" <- 1]["x" <- 2]) = false := rfl
+  rw [hs, hcond]
+  simp
+  apply ReflTrans.refl
 
 theorem star.cat_skip_cat
   (hc: (c, s) ~>* (skip, s')):
   (c++c', s) ~>* (skip++c', s') :=
-  ReflTrans.lift (fun (c, s) => (c++c', s)) (fun h => cat h) hc
+  ReflTrans.lift (fun (c, s) => (c++c', s)) (cat .) hc
 
 theorem star.cat
   (hc: (c, s) ~>* (skip, s'))
